theories/zoo_saturn/mpsc_queue_1__opaque.v
@@ -1,8 +1,0 @@
-Require Import zoo_saturn.mpsc_queue_1__code.
-
-#[global] Opaque mpsc_queue_1٠create.
-#[global] Opaque mpsc_queue_1٠is_empty.
-#[global] Opaque mpsc_queue_1٠push₁.
-#[global] Opaque mpsc_queue_1٠fix_back.
-#[global] Opaque mpsc_queue_1٠push.
-#[global] Opaque mpsc_queue_1٠pop.
